# Origin
$f(x)=f(x_0)+f'(x_0)(x-x_0)+\frac{f''(x_0)}{2!}(x-x_0)^2+...+O((x-x_0)^n)$
# x=0
$f(x)=f(0)+f'(0)x+\frac{f''(0)}{2!}x^2+...+O(x^n)$
->
$sin(x)=sin0+cos0*x-\frac{sin0}{2!}x^2-\frac{cos0}{3!}x^3+\frac{sin0}{4!}x^4+...+o(x^n)$
$cos(x)=cos0-sin0*x-\frac{cos0}{2!}x^2+\frac{sin0}{3!}x^4+\frac{cos0}{4!}x^4+...+O(x^n)$
# Formula
$sin(x)=x-\frac{x^3}{3!}+\frac{x^5}{5!}+...+(-1)^{n-1}\frac{x^{2n-1}}{(2n-1)!}+...+O(x^{2n-1})$
$cos(x)=1-\frac{x^2}{2!}+...+(-1)^n\frac{x^{2n}}{(2n)!}+O(n^2n)$
$e^x=1+x+\frac{x^2}{2!}+...+\frac{x^n}{n!}+O(x^n)$
$ln(1+x)=x-\frac{x^2}{2}+...+(-1)^{n-1}\frac{x^n}{n}+O(x^n)$
$(1+x)^a=1+ax+\frac{a(a-1)}{2!}x^2+...+\frac{a(a-1)...(a-n+1)}{n!}x^n+O(x^n)$